wip: defining the Eff effect and handlers that respect equations

Eff.fst
@@ -1,5 +1,190 @@
 module Eff
 
+open Eff.Signature
+
+module T = Eff.Template
+
+open Eff.Template.Equation
+
+module L = FStar.List.Tot
+
+(* Equation annotations in computation types *)
+
+let equations ops = list (equation ops)
+
+
+(* Subtyping equation annotations *)
+
+let eq_subcomp #ops1 #ops2 (eq:equation ops1)
+  : Pure (equation ops2)
+         (requires (ops1 `sub` ops2))
+         (ensures  (fun _ -> True))
+  = {
+      vctx = eq.vctx;
+      cctx = eq.cctx;
+      lhs  = (fun vvars -> eq.lhs vvars);
+      rhs  = (fun vvars -> eq.rhs vvars)
+    }
+
+let eqs_sub #ops1 #ops2 (eqs1:equations ops1) (eqs2:equations ops2)
+  = ops1 `sub` ops2 /\
+    (forall (eq:equation ops1) . L.memP eq eqs1 ==> L.memP (eq_subcomp eq) eqs2)
+
+
+(* Computation tree representation of the Eff effect *)
+
+let eff (a:Type u#a) (ops:sig) (eqs:equations ops)
+  = T.template a ops
+
+
+(* Monadic operators on the Eff effect *)
+
+let eff_return a x #ops #eqs
+  : eff a ops eqs
+  = T.template_return a x #ops
+
+let eff_bind a b #ops #eqs
+  (t1:eff a ops eqs) 
+  (t2:a -> eff b ops eqs) 
+  : eff b ops eqs
+  = T.template_bind a b #ops t1 t2
+
+let eff_subcomp a #ops1 #ops2 #eqs1 #eqs2
+  (t:eff a ops1 eqs1)
+  : Pure (eff a ops2 eqs2)
+         (requires (ops1 == ops2 /\ eqs1 === eqs2)) // temporarily, TODO: find way around the typechecking problems with inclusions
+         //(requires (ops1 `sub` ops2 /\ eqs1 `eqs_sub` eqs2))
+         (ensures (fun _ -> True))
+  = T.template_subcomp a #ops1 #ops2 t
+
+let eff_if_then_else a #ops #eqs
+  (f:eff a ops eqs)
+  (g:eff a ops eqs)
+  (b:bool)
+  : Type
+  = eff a ops eqs
+
+let eff_perform #ops #eqs
+  (op:op{op `mem` ops})
+  (x:param_of op)
+  : eff (arity_of op) ops eqs
+  = T.Node op x (fun y -> T.Leaf y)
+
+
+(* The Eff effect *)
+
+[@@allow_informative_binders]
+total
+reifiable
+reflectable
+layered_effect {
+  Eff : a:Type -> ops:sig -> equations ops -> Effect
+  with
+  repr         = eff;
+  return       = eff_return;
+  bind         = eff_bind;
+  subcomp      = eff_subcomp;
+  if_then_else = eff_if_then_else;
+  perform      = eff_perform
+}
+
+
+(* Lifting of pure computations into the Eff effect *)
+
+let lift_pure_eff a wp ops eqs
+  (f:eqtype_as_type unit -> PURE a wp)
+  : Pure (eff a ops eqs)
+         (requires (wp (fun _ -> True)))
+         (ensures (fun _ -> True))
+  = FStar.Monotonic.Pure.elim_pure_wp_monotonicity wp;
+    T.Leaf (f ())
+
+sub_effect PURE ~> Eff = lift_pure_eff
+
+
+(* Empty signature computations are pure *)
+
+let eff_emp_pure #a (c:unit -> eff a emp []) : a 
+  = match c () with
+    | T.Leaf x -> x
+  
+let emp_pure #a (c:unit -> Eff a emp []) : a 
+  = eff_emp_pure (fun x -> reify (c ()))
+
+
+(* Performing an algebraic effect *)
+
+let perform #ops #eqs (op:op{op `mem` ops}) (x:param_of op) 
+  : Eff (arity_of op) ops eqs
+  = Eff?.perform op x
+
+
+(* Effect handlers (on Eff effect representations) *)
+
+let raw_eff_handler (ops:sig) (eqs:equations ops) (a:Type) (ops':sig) (eqs':equations ops') 
+  = op:op{op `mem` ops} -> param_of op -> (arity_of op -> eff a ops' eqs') -> eff a ops' eqs'
+
+let rec to_respects_hypotheses a #ops (eqs:equations ops) 
+  : Type0
+  = match eqs with
+    | [] -> True
+    | eq :: eqs' ->
+      eq_to_prop (to_inst_equation (to_template_equation eq) (T.id_template_handler a ops))
+      /\
+      to_respects_hypotheses a eqs'
+
+let rec to_respects_conclusion #a #ops #ops' (eqs:equations ops) #eqs' (h:raw_eff_handler ops eqs a ops' eqs')
+  : Type0
+  = match eqs with
+    | [] -> unit
+    | eq :: eqs'' -> 
+        _:unit{eq_to_prop (to_inst_equation (to_template_equation eq) h)}
+        *
+        to_respects_conclusion eqs'' h
+
+let eff_respects #a #ops #ops' #eqs #eqs' (h:raw_eff_handler ops eqs a ops' eqs') 
+  (proofs:norm [delta;zeta;primops;simplify;iota] (to_respects_conclusion eqs h))
+  : unit -> norm [delta;zeta;primops;simplify;iota] (to_respects_conclusion eqs h)
+  = fun _ -> proofs
+
+let eff_handler_respects (ops:sig) (eqs:equations ops) (a:Type) (ops':sig) (eqs':equations ops') (h:raw_eff_handler ops eqs a ops' eqs') =
+  unit -> Pure (norm [delta;zeta;primops;simplify;iota] (to_respects_conclusion eqs h))
+              (requires (norm [delta;zeta;primops;simplify;iota] (to_respects_hypotheses a eqs')))
+              (ensures  (fun _ -> True))
+
+let eff_handler (ops:sig) (eqs:equations ops) (a:Type) (ops':sig) (eqs':equations ops')
+  = h:raw_eff_handler ops eqs a ops' eqs'
+    & 
+    norm [delta;zeta;primops;simplify;iota] (eff_handler_respects ops eqs a ops' eqs' h)
+
+
+
+
+
+
+
+
+
+
+
+
+
+(*
+let handler (ops:S.sig) (a:Type) (ops':S.sig) = 
+  op:S.op{op `S.mem` ops} -> S.param_of op -> (S.arity_of op -> Eff a ops') -> Eff a ops'
+
+let reflect_cont #a #b #ops (k:b -> eff_repr a ops) (y:b) : Eff a ops
+  = Eff?.reflect (k y)
+
+let to_eff_handler #ops #a #ops'
+  (h:handler ops a ops')
+  : eff_handler ops a ops'
+  = fun op x k ->  
+      (reify (h op x (reflect_cont k))) 
+*)
+
+
+(*
 module S = Eff.Signature
 
 (* Computation tree representation of the Eff effect *)
@@ -146,3 +331,5 @@ let handle #a #b #ops #ops'
         (reify (f ()))
         (to_eff_handler h)
         (fun x -> reify (k x)))
+
+*)
