Eff.Equation.Test.fst
@@ -1,0 +1,91 @@
+module Eff.Equation.Test
+
+open Eff.Signature
+open Eff.Template.Equation
+
+module T = Eff.Template
+
+open Eff
+
+(* Read and write effects for integer state *)
+
+let read = Op "read" #unit #int
+let write = Op "write" #int #unit
+
+let r : sig = singleton read
+let w : sig = singleton write
+let rw : sig = r `union` w
+
+
+(* State equations using templates *)
+
+let st_eq1 : equation rw 
+  = { 
+      vctx = [];
+      cctx = [unit];
+      lhs  = (fun vvars -> let y = T.perform read () in 
+                        let y' = T.perform write y in
+                        cvar 0 y');
+      rhs  = (fun vvars -> cvar 0 ())
+    }
+
+let st_eq2 : equation rw
+  = {
+      vctx = [int];
+      cctx = [int];
+      lhs  = (fun vvars -> T.perform write (vvar vvars 0);
+                        let y = T.perform read () in
+                        cvar 0 y);
+      rhs  = (fun vvars -> T.perform write (vvar vvars 0);
+                        cvar 0 (vvar vvars 0))
+    }
+
+let st_eq3 : equation rw
+  = {
+      vctx = [int;int];
+      cctx = [unit];
+      lhs  = (fun vvars -> T.perform write (vvar vvars 0);
+                        let y = T.perform write (vvar vvars 1) in
+                        cvar 0 y);
+      rhs  = (fun vvars -> let y = T.perform write (vvar vvars 1) in
+                        cvar 0 y)
+    }
+
+
+
+(* ************************** *)
+
+
+let st_eq : equation rw
+  = {
+      vctx = [int;int;int];
+      cctx = [unit];
+      lhs  = (fun vvars -> T.perform write (vvar vvars 0);
+                        T.perform write (vvar vvars 1);
+                        let y = T.perform write (vvar vvars 2) in
+                        cvar 0 y);
+      rhs  = (fun vvars -> T.perform write (vvar vvars 0);
+                        let y = T.perform write (vvar vvars 2) in
+                        cvar 0 y)
+    }
+
+
+(* ************************** *)
+
+assume val t : Type0
+
+
+let h1_raw : raw_eff_handler rw [] t rw []
+  = fun op x k -> T.Node op x k
+
+let h1 : eff_handler rw [] t rw []
+  = (| h1_raw , eff_respects h1_raw () |)
+
+
+let h2_raw : raw_eff_handler rw [] t rw [st_eq3]
+  = fun op x k -> T.Node op x k
+
+(*
+let h2 : eff_handler rw [] t rw [st_eq3]
+  = (| h2_raw , eff_respects h2_raw () |)
+*)
